books/centaur/fgl/interp-st.lisp
@@ -52,7 +52,8 @@
    (intro-synvars booleanp :default t)
    (simplify-logic booleanp :default t)
    (trace-rewrites booleanp :default nil)
-   (make-ites booleanp :default nil)))
+   (make-ites booleanp :default nil)
+   (branch-on-ifs booleanp :default t)))
 
 (local (defthm unsigned-byte-p-of-flags
          (implies (interp-flags-p flags)
